@prefix : <http://www.modsem.org/fakt-news#> .
@prefix fn: <http://www.modsem.org/fakt-news#> .
@prefix dct: <http://purl.org/dc/terms/> .
@prefix owl: <http://www.w3.org/2002/07/owl#> .
@prefix rdf: <http://www.w3.org/1999/02/22-rdf-syntax-ns#> .
@prefix xml: <http://www.w3.org/XML/1998/namespace> .
@prefix xsd: <http://www.w3.org/2001/XMLSchema#> .
@prefix foaf: <http://xmlns.com/foaf/0.1/> .
@prefix obda: <https://w3id.org/obda/vocabulary#> .
@prefix prov: <http://www.w3.org/ns/prov#> .
@prefix rdfs: <http://www.w3.org/2000/01/rdf-schema#> .
@prefix skos: <http://www.w3.org/2004/02/skos/core#> .
@prefix vann: <http://purl.org/vocab/vann/> .
@prefix schema: <http://schema.org/> .
@prefix dcterms: <http://purl.org/dc/terms/> .
@base <http://www.modsem.org/fakt-news> .

<http://www.modsem.org/fakt-news> rdf:type owl:Ontology ;
                                   owl:imports <http://www.ontologydesignpatterns.org/cp/owl/set.owl> ,
                                               <http://www.ontologydesignpatterns.org/cp/owl/timeinterval.owl> ;
                                   dcterms:creator "Lorenzo Tabasso"@it ,
                                                   "Pio Raffaele Fina"@it ;
                                   dcterms:date "2021-03-05" ;
                                   dcterms:description "An Ontology to describe and annotate the fact checking process."@en ;
                                   vann:preferredNamespacePrefix "fn"@en ;
                                   vann:preferredNamespaceUri "http://www.modsem.org/fakt-news"@en ;
                                   rdfs:label "Fakt News"@en .

#################################################################
#    Annotation properties
#################################################################

###  http://purl.org/dc/terms/creator
dcterms:creator rdf:type owl:AnnotationProperty ;
                rdfs:comment "An entity responsible for making the resource."@en ;
                rdfs:label "creator"@en .


###  http://purl.org/dc/terms/date
dcterms:date rdf:type owl:AnnotationProperty .


###  http://purl.org/dc/terms/description
dcterms:description rdf:type owl:AnnotationProperty ;
                    rdfs:comment "An account of the resource."@en ;
                    rdfs:label "description"@en .


###  http://purl.org/vocab/vann/preferredNamespacePrefix
vann:preferredNamespacePrefix rdf:type owl:AnnotationProperty ;
                              rdfs:comment "The preferred namespace prefix to use when using terms from this vocabulary in an XML document."@en ;
                              rdfs:label "preferredNamespacePrefix"@en .


###  http://purl.org/vocab/vann/preferredNamespaceUri
vann:preferredNamespaceUri rdf:type owl:AnnotationProperty ;
                           rdfs:comment "The preferred namespace URI to use when using terms from this vocabulary in an XML document."@en ;
                           rdfs:label "preferredNamespaceUri"@en .


###  http://www.ontologydesignpatterns.org/cp/owl/collectionentity.owl#hasMember
<http://www.ontologydesignpatterns.org/cp/owl/collectionentity.owl#hasMember> rdf:type owl:AnnotationProperty .


###  http://www.ontologydesignpatterns.org/cp/owl/collectionentity.owl#isMemberOf
<http://www.ontologydesignpatterns.org/cp/owl/collectionentity.owl#isMemberOf> rdf:type owl:AnnotationProperty .


###  http://www.w3.org/2004/02/skos/core#altLabel
skos:altLabel rdf:type owl:AnnotationProperty .


###  http://www.w3.org/2004/02/skos/core#example
skos:example rdf:type owl:AnnotationProperty .


#################################################################
#    Datatypes
#################################################################

###  http://www.w3.org/2001/XMLSchema#date
xsd:date rdf:type rdfs:Datatype .


#################################################################
#    Object Properties
#################################################################

###  http://www.modsem.org/fakt-news#affiliatedTo
fn:affiliatedTo rdf:type owl:ObjectProperty ;
                rdfs:domain prov:Agent ;
                rdfs:range prov:Agent ;
                rdfs:comment "An affiliation bond between a Fact Checker and a Organization."@en ;
                rdfs:label "affiliated to"@en .


###  http://www.modsem.org/fakt-news#associatedReview
fn:associatedReview rdf:type owl:ObjectProperty ;
                    rdfs:subPropertyOf owl:topObjectProperty ;
                    owl:inverseOf fn:claimReviewed ;
                    rdfs:domain fn:Claim ;
                    rdfs:range fn:Review ;
                    rdfs:comment "A link between a Claim and a Review about it."@en ;
                    rdfs:label "associated review"@en .


###  http://www.modsem.org/fakt-news#claimReviewed
fn:claimReviewed rdf:type owl:ObjectProperty ;
                 rdfs:subPropertyOf owl:topObjectProperty ;
                 rdfs:domain fn:Review ;
                 rdfs:range fn:Claim ;
                 owl:propertyChainAxiom ( fn:wasOutputOfClaimEvaluation
                                          fn:hasPreviousActivity
                                          prov:used
                                        ) ;
                 rdfs:comment "Inverse of associated review. It rapresent a link between a review and the claim which is reviewed."@en ;
                 rdfs:label "claim reviewed"@en .


###  http://www.modsem.org/fakt-news#create
fn:create rdf:type owl:ObjectProperty ;
          owl:inverseOf fn:creator ;
          rdfs:comment "Inverse propriety of dct:creator. Used in order to define createCodeOfPrinciple object proprierty."@en ;
          rdfs:label "create"@en .


###  http://www.modsem.org/fakt-news#createCodeOfPrinciples
fn:createCodeOfPrinciples rdf:type owl:ObjectProperty ;
                          rdfs:subPropertyOf fn:create ;
                          rdfs:domain fn:FactCheckingAuthority ;
                          rdfs:range fn:CodeOfPrinciples ;
                          rdfs:comment "Denotes the creation of a code of principles by a Fact Checking Authority."@en ;
                          rdfs:label "create code of principles"@en .


###  http://www.modsem.org/fakt-news#creator
fn:creator rdf:type owl:ObjectProperty ;
           rdfs:subPropertyOf prov:wasAttributedTo ;
           rdfs:domain schema:CreativeWork ;
           rdfs:comment "Denotes the entity who creates the resource."@en ;
           rdfs:label "creator"@en .


###  http://www.modsem.org/fakt-news#derivedFromSource
fn:derivedFromSource rdf:type owl:ObjectProperty ;
                     rdfs:subPropertyOf prov:wasAttributedTo ;
                     owl:inverseOf fn:isSourceOfEvidence ;
                     rdfs:domain fn:Evidence ;
                     rdfs:range fn:EvidenceSource ;
                     rdfs:comment "Denotes the link between the Evidence (i.e. the actual fact) and the Evidence Source."@en ;
                     rdfs:label "derived from source"@en .


###  http://www.modsem.org/fakt-news#hasActivity
fn:hasActivity rdf:type owl:ObjectProperty ;
               owl:inverseOf fn:isActivityOfPlan ;
               rdf:type owl:InverseFunctionalProperty ;
               rdfs:domain prov:Plan ;
               rdfs:range prov:Activity ;
               rdfs:comment "Denotes the membership of an Activity to a Plan."@en ;
               rdfs:label "has activity"@en .


###  http://www.modsem.org/fakt-news#hasEvidence
fn:hasEvidence rdf:type owl:ObjectProperty ;
               rdfs:domain fn:Review ;
               rdfs:range fn:Evidence ;
               rdfs:label "Bond from a Review to a Evidence."@en ,
                          "has evidence"@en .


###  http://www.modsem.org/fakt-news#hasJudgment
fn:hasJudgment rdf:type owl:ObjectProperty ;
               rdfs:domain fn:Review ;
               rdfs:range fn:Judgment ;
               rdfs:comment "Represent the Judgment inside a Review about a Claim."@en ;
               rdfs:label "has judgment"@en .


###  http://www.modsem.org/fakt-news#hasNextActivity
fn:hasNextActivity rdf:type owl:ObjectProperty ;
                   rdfs:subPropertyOf owl:topObjectProperty ;
                   owl:inverseOf fn:hasPreviousActivity ;
                   rdf:type owl:TransitiveProperty ;
                   rdfs:domain prov:Activity ;
                   rdfs:range prov:Activity ;
                   rdfs:comment "Points to the next activity after the current one in a plan."@en ;
                   rdfs:label "has next activity"@en .


###  http://www.modsem.org/fakt-news#hasPreviousActivity
fn:hasPreviousActivity rdf:type owl:ObjectProperty ;
                       rdfs:subPropertyOf owl:topObjectProperty ;
                       rdf:type owl:TransitiveProperty ;
                       rdfs:domain prov:Activity ;
                       rdfs:range prov:Activity ;
                       rdfs:comment "Points to the activity prior to the current one in a plan."@en ;
                       rdfs:label "has previous activity"@en .


###  http://www.modsem.org/fakt-news#hasRating
fn:hasRating rdf:type owl:ObjectProperty ,
                      owl:FunctionalProperty ;
             rdfs:domain fn:Review ;
             rdfs:range fn:Rating ;
             rdfs:comment "Represent the Rating inside a Review about a Claim."@en ;
             rdfs:label "has rating"@en .


###  http://www.modsem.org/fakt-news#hasTimeInterval
fn:hasTimeInterval rdf:type owl:ObjectProperty ;
                   rdfs:domain prov:Activity ;
                   rdfs:range <http://www.ontologydesignpatterns.org/cp/owl/timeinterval.owl#TimeInterval> ;
                   rdfs:comment "It represents the link between an activity and the time interval in which it occurs."@en ;
                   rdfs:label "has time interval"@en .


###  http://www.modsem.org/fakt-news#isActivityOfPlan
fn:isActivityOfPlan rdf:type owl:ObjectProperty ,
                             owl:FunctionalProperty ;
                    rdfs:domain prov:Activity ;
                    rdfs:range prov:Plan ;
                    rdfs:comment "It represents the link between an activity and the plan of which it is part."@en ;
                    rdfs:label "is activity of plan"@en .


###  http://www.modsem.org/fakt-news#isCertificatedBy
fn:isCertificatedBy rdf:type owl:ObjectProperty ;
                    rdfs:domain fn:FactCheckingOrganization ;
                    rdfs:range fn:FactCheckingAuthority ;
                    owl:propertyChainAxiom ( fn:observeCodeOfPrinciples
                                             fn:creator
                                           ) ;
                    rdfs:comment "indicates that a Fact Checking Organization is certified by a Fact Checking Authority (i.e. it follows the principles defined by the Fact Checking AUthority)."@en ;
                    rdfs:label "is certified by"@en .


###  http://www.modsem.org/fakt-news#isClaimedBy
fn:isClaimedBy rdf:type owl:ObjectProperty ;
               rdfs:subPropertyOf fn:creator ;
               rdfs:domain fn:Claim ;
               rdfs:comment "Sub-property of creator. Denotes the claimant of a Claim."@en ;
               rdfs:label "is claimed by"@en .


###  http://www.modsem.org/fakt-news#isFirstActivityOfPlan
fn:isFirstActivityOfPlan rdf:type owl:ObjectProperty ;
                         rdfs:subPropertyOf fn:isActivityOfPlan ;
                         rdfs:comment "It represents the first activity of the plan."@en ;
                         rdfs:label "is first activity of plan"@en .


###  http://www.modsem.org/fakt-news#isLastActivityOfPlan
fn:isLastActivityOfPlan rdf:type owl:ObjectProperty ;
                        rdfs:subPropertyOf fn:isActivityOfPlan ;
                        rdfs:comment "It represents the last activity of the plan."@en ;
                        rdfs:label "is last activity of plan"@en .


###  http://www.modsem.org/fakt-news#isReviewedBy
fn:isReviewedBy rdf:type owl:ObjectProperty ;
                rdfs:subPropertyOf fn:creator ;
                rdfs:domain fn:Review ;
                rdfs:comment "Sub-property of creator. Denotes the reviewer of a Review."@en ;
                rdfs:label "is reviewed by"@en .


###  http://www.modsem.org/fakt-news#isSourceOfEvidence
fn:isSourceOfEvidence rdf:type owl:ObjectProperty ;
                      rdfs:comment "Used to denote that a Source of Evidence actually becomes the source of an Evidence."@en ;
                      rdfs:label "is source of evidence"@en .


###  http://www.modsem.org/fakt-news#isUsedByClaimEvaluation
fn:isUsedByClaimEvaluation rdf:type owl:ObjectProperty ;
                           rdfs:subPropertyOf prov:used ;
                           rdfs:domain fn:ClaimEvaluationActivity ;
                           rdfs:range fn:Evidence ;
                           rdfs:comment "Sub-property of prov:used to indicate the use (as input) of Evidence in the Claim Evaluation Activity."@en ;
                           rdfs:label "is used by claim evaluation"@en .


###  http://www.modsem.org/fakt-news#isUsedBySelection
fn:isUsedBySelection rdf:type owl:ObjectProperty ;
                     rdfs:subPropertyOf prov:used ;
                     rdfs:domain fn:SelectionActivity ;
                     rdfs:range fn:AlternativesSet ;
                     rdfs:comment "Sub-property of prov:used to indicate the use (as input) of Alternative Set in the Selection Activity."@en ;
                     rdfs:label "is used by selection"@en .


###  http://www.modsem.org/fakt-news#isUsedByVerification
fn:isUsedByVerification rdf:type owl:ObjectProperty ;
                        rdfs:subPropertyOf prov:used ;
                        rdfs:domain fn:VerificationActivity ;
                        rdfs:range fn:Claim ;
                        rdfs:comment "Sub-property of prov:used to indicate the use (as input) of Claim in the Verification Activity."@en ;
                        rdfs:label "is used by verification"@en .


###  http://www.modsem.org/fakt-news#observeCodeOfPrinciples
fn:observeCodeOfPrinciples rdf:type owl:ObjectProperty ;
                           rdfs:domain fn:FactCheckingOrganization ;
                           rdfs:range fn:CodeOfPrinciples ;
                           rdfs:comment "Object property asserted when an authority verifies that its principles are being observed."^^xsd:string ;
                           rdfs:label "observe code of principles"@en ;
                           skos:example "https://www.poynter.org/ifcn-fact-checkers-code-of-principles/"@en .


###  http://www.modsem.org/fakt-news#supportedBy
fn:supportedBy rdf:type owl:ObjectProperty ;
               rdfs:domain fn:Evidence ;
               rdfs:range fn:DigitalDocument ;
               rdfs:comment "A review is supported by a materialization of some sort of document (for example a subtype of creative work)."@en ;
               rdfs:label "supported by"@en .


###  http://www.modsem.org/fakt-news#wasOutputOfClaimEvaluation
fn:wasOutputOfClaimEvaluation rdf:type owl:ObjectProperty ;
                              rdfs:subPropertyOf prov:wasGeneratedBy ;
                              rdfs:domain fn:Review ;
                              rdfs:range fn:ClaimEvaluationActivity ;
                              rdfs:comment "Sub-property of prov:wasGeneratedBy indicating the output of the Claim Evaluation Activity, that is, the Review."@en ;
                              rdfs:label "was output of claim evaluation"@en .


###  http://www.modsem.org/fakt-news#wasOutputOfSelection
fn:wasOutputOfSelection rdf:type owl:ObjectProperty ;
                        rdfs:subPropertyOf prov:wasGeneratedBy ;
                        rdfs:domain fn:Claim ;
                        rdfs:range fn:SelectionActivity ;
                        rdfs:comment "Sub-property of prov:wasGeneratedBy indicating the output of the Selection Activity, that is, the Claim."@en ;
                        rdfs:label "was output of selection"@en .


###  http://www.modsem.org/fakt-news#wasOutputOfVerification
fn:wasOutputOfVerification rdf:type owl:ObjectProperty ;
                           rdfs:subPropertyOf prov:wasGeneratedBy ;
                           rdfs:domain fn:Evidence ;
                           rdfs:range fn:VerificationActivity ;
                           rdfs:comment "Sub-property of prov:wasGeneratedBy indicating the output of the Verification Activity, that is, the Evidence."@en ;
                           rdfs:label "was output of verfication"@en .


###  http://www.w3.org/ns/prov#agent
prov:agent rdf:type owl:ObjectProperty ;
           rdfs:domain prov:Association ;
           rdfs:range prov:Agent ;
           rdfs:comment "The prov:agent property references an prov:Agent which influenced a resource. This property applies to an prov:AgentInfluence, which is given by a subproperty of prov:qualifiedInfluence from the influenced prov:Entity, prov:Activity or prov:Agent."@en ;
           rdfs:label "agent"@en ;
           skos:example "https://www.w3.org/TR/prov-o/#p_agent"@en .


###  http://www.w3.org/ns/prov#hadRole
prov:hadRole rdf:type owl:ObjectProperty ;
             rdfs:domain prov:Association ;
             rdfs:range prov:Role ;
             rdfs:comment "A role is the function of an entity or agent with respect to an activity, in the context of a usage, generation, invalidation, association, start, and end."@en ;
             rdfs:label "had role"@en ;
             skos:example "https://www.w3.org/TR/prov-o/#hadRole"@en .


###  http://www.w3.org/ns/prov#qualifiedAssociation
prov:qualifiedAssociation rdf:type owl:ObjectProperty ;
                          rdfs:domain prov:Activity ;
                          rdfs:range prov:Association ;
                          rdfs:comment "An activity association is an assignment of responsibility to an agent for an activity, indicating that the agent had a role in the activity. It further allows for a plan to be specified, which is the plan intended by the agent to achieve some goals in the context of this activity."@en ;
                          rdfs:label "qualified association"@en ;
                          skos:example "https://www.w3.org/TR/prov-o/#qualifiedAssociation"@en .


###  http://www.w3.org/ns/prov#used
prov:used rdf:type owl:ObjectProperty ;
          rdfs:domain prov:Activity ;
          rdfs:range prov:Entity ;
          rdfs:comment "Usage is the beginning of utilizing an entity by an activity. Before usage, the activity had not begun to utilize this entity and could not have been affected by the entity."@en ;
          rdfs:label "used"@en ;
          skos:example "https://www.w3.org/TR/prov-o/#used"@en .


###  http://www.w3.org/ns/prov#wasAssociatedWith
prov:wasAssociatedWith rdf:type owl:ObjectProperty ;
                       rdfs:domain prov:Activity ;
                       rdfs:range prov:Agent ;
                       rdfs:comment "An activity association is an assignment of responsibility to an agent for an activity, indicating that the agent had a role in the activity. It further allows for a plan to be specified, which is the plan intended by the agent to achieve some goals in the context of this activity."@en ;
                       rdfs:label "was associated with"@en ;
                       skos:example "https://www.w3.org/TR/prov-o/#wasAssociatedWith"@en .


###  http://www.w3.org/ns/prov#wasAttributedTo
prov:wasAttributedTo rdf:type owl:ObjectProperty ;
                     rdfs:domain prov:Entity ;
                     rdfs:range prov:Agent ;
                     rdfs:comment "Attribution is the ascribing of an entity to an agent."@en ;
                     rdfs:label "was attributed to"@en ;
                     skos:example "https://www.w3.org/TR/prov-o/#wasAttributedTo"@en .


###  http://www.w3.org/ns/prov#wasGeneratedBy
prov:wasGeneratedBy rdf:type owl:ObjectProperty ;
                    rdfs:subPropertyOf owl:topObjectProperty ;
                    rdfs:domain prov:Entity ;
                    rdfs:range prov:Activity ;
                    rdfs:comment "Generation is the completion of production of a new entity by an activity. This entity did not exist before generation and becomes available for usage after this generation."@en ;
                    rdfs:label "was generated by"@en ;
                    skos:example "https://www.w3.org/TR/prov-o/#wasGeneratedBy"@en .


#################################################################
#    Data properties
#################################################################

###  http://purl.org/dc/terms/date
dcterms:date rdf:type owl:DatatypeProperty .


###  http://purl.org/dc/terms/language
dcterms:language rdf:type owl:DatatypeProperty ;
                 rdfs:domain schema:CreativeWork ;
                 rdfs:range xsd:string ;
                 rdfs:comment "A language of the resource."@en ;
                 rdfs:label "language"@en .


###  http://purl.org/dc/terms/title
dcterms:title rdf:type owl:DatatypeProperty ;
              rdfs:subPropertyOf owl:topDataProperty ;
              rdfs:comment "A name given to the resource."@en ;
              rdfs:label "title"@en .


###  http://schema.org/name
schema:name rdf:type owl:DatatypeProperty ;
            rdfs:range xsd:string ;
            rdfs:comment "The name of the item."@en ;
            rdfs:label "name"@en .


###  http://schema.org/url
schema:url rdf:type owl:DatatypeProperty ;
           rdfs:range xsd:anyURI ;
           rdfs:comment "The URL of an item."@en ;
           rdfs:label "url"@en ;
           skos:altLabel "URL"@en .


###  http://www.modsem.org/fakt-news#capacityType
fn:capacityType rdf:type owl:DatatypeProperty ;
                rdfs:domain fn:EvidenceSource ;
                rdfs:range [ rdf:type rdfs:Datatype ;
                             owl:oneOf [ rdf:type rdf:List ;
                                         rdf:first "Citizen" ;
                                         rdf:rest [ rdf:type rdf:List ;
                                                    rdf:first "Civil Service" ;
                                                    rdf:rest [ rdf:type rdf:List ;
                                                               rdf:first "Company" ;
                                                               rdf:rest [ rdf:type rdf:List ;
                                                                          rdf:first "Expert" ;
                                                                          rdf:rest [ rdf:type rdf:List ;
                                                                                     rdf:first "Government" ;
                                                                                     rdf:rest [ rdf:type rdf:List ;
                                                                                                rdf:first "Lobby" ;
                                                                                                rdf:rest [ rdf:type rdf:List ;
                                                                                                           rdf:first "NGO" ;
                                                                                                           rdf:rest [ rdf:type rdf:List ;
                                                                                                                      rdf:first "Opposition" ;
                                                                                                                      rdf:rest [ rdf:type rdf:List ;
                                                                                                                                 rdf:first "Think Tank" ;
                                                                                                                                 rdf:rest rdf:nil
                                                                                                                               ]
                                                                                                                    ]
                                                                                                         ]
                                                                                              ]
                                                                                   ]
                                                                        ]
                                                             ]
                                                  ]
                                       ]
                           ] ;
                rdfs:comment "The Evidence Source social function indipendent of the context."@en ;
                rdfs:label "capacity"@en ;
                skos:altLabel "Position"@en .


###  http://www.modsem.org/fakt-news#claimContent
fn:claimContent rdf:type owl:DatatypeProperty ;
                rdfs:subPropertyOf fn:documentContent ;
                rdfs:domain fn:Claim ;
                rdfs:range xsd:string ;
                rdfs:comment "The main content of a claim: what claimant said."@en ;
                rdfs:label "claim content"@en .


###  http://www.modsem.org/fakt-news#documentContent
fn:documentContent rdf:type owl:DatatypeProperty ;
                   rdfs:domain fn:DigitalDocument ;
                   rdfs:comment "The main content of the digital document."@en ;
                   rdfs:label "document content"@en .


###  http://www.modsem.org/fakt-news#judgmentSummary
fn:judgmentSummary rdf:type owl:DatatypeProperty ;
                   rdfs:domain fn:Judgment ;
                   rdfs:range xsd:string ;
                   rdfs:comment "A brief description of the judgment given by some fact checker."@en ;
                   rdfs:label "judgment summary"@en ;
                   skos:altLabel "judgment description"@en .


###  http://www.modsem.org/fakt-news#mention
fn:mention rdf:type owl:DatatypeProperty ;
           rdfs:domain fn:Review ;
           rdfs:range xsd:string ;
           rdfs:comment "A mention to some entity in a review."@en ;
           rdfs:label "mention"@en .


###  http://www.modsem.org/fakt-news#ratingAssociatedMedia
fn:ratingAssociatedMedia rdf:type owl:DatatypeProperty ;
                         rdfs:domain fn:Rating ;
                         rdfs:range xsd:anyURI ;
                         rdfs:comment "A visual representation of the rating value."@en ;
                         rdfs:label "rating associated media"@en ;
                         skos:altLabel "rating depiction"@en .


###  http://www.modsem.org/fakt-news#ratingSystemComment
fn:ratingSystemComment rdf:type owl:DatatypeProperty ;
                       rdfs:domain fn:Rating ;
                       rdfs:range xsd:string ;
                       rdfs:comment "A comment on the rating system."@en ;
                       rdfs:label "rating system comment"@en .


###  http://www.modsem.org/fakt-news#ratingValue
fn:ratingValue rdf:type owl:DatatypeProperty ;
               rdfs:domain fn:Rating ;
               rdfs:range [ rdf:type rdfs:Datatype ;
                            owl:oneOf [ rdf:type rdf:List ;
                                        rdf:first "False" ;
                                        rdf:rest [ rdf:type rdf:List ;
                                                   rdf:first "Mostly False" ;
                                                   rdf:rest [ rdf:type rdf:List ;
                                                              rdf:first "Mostly True" ;
                                                              rdf:rest [ rdf:type rdf:List ;
                                                                         rdf:first "True" ;
                                                                         rdf:rest rdf:nil
                                                                       ]
                                                            ]
                                                 ]
                                      ]
                          ] ;
               rdfs:comment "The rating value that encode a final verdict about the claim truthfulness."@en ;
               rdfs:label "rating value"@en .


###  http://www.modsem.org/fakt-news#reviewContent
fn:reviewContent rdf:type owl:DatatypeProperty ;
                 rdfs:subPropertyOf fn:documentContent ;
                 rdfs:domain fn:Review ;
                 rdfs:range xsd:string ;
                 rdfs:comment "The content of a review article."@en ;
                 rdfs:label "review content"@en .


###  http://www.modsem.org/fakt-news#tag
fn:tag rdf:type owl:DatatypeProperty ;
       rdfs:domain fn:Review ;
       rdfs:comment "A topic tag of the review."@en ;
       rdfs:label "tag"@en ;
       skos:altLabel "topic tag"@en .


#################################################################
#    Classes
#################################################################

###  http://schema.org/CreativeWork
schema:CreativeWork rdf:type owl:Class ;
                    owl:equivalentClass fn:DigitalDocument ;
                    rdfs:subClassOf prov:Entity ;
                    rdfs:comment "The most generic kind of creative work, including books, movies, photographs, software programs, etc."@en ;
                    rdfs:label "Creative Work"@en .


###  http://www.modsem.org/fakt-news#AlternativesSet
fn:AlternativesSet rdf:type owl:Class ;
                   rdfs:subClassOf <http://www.ontologydesignpatterns.org/cp/owl/set.owl#Set> ;
                   rdfs:comment "A set of claims from which the fact-checker chooses the claim to verify."@en ;
                   rdfs:label "Alternatives Set"@en .


###  http://www.modsem.org/fakt-news#Author
fn:Author rdf:type owl:Class ;
          owl:equivalentClass [ rdf:type owl:Class ;
                                owl:unionOf ( fn:Claimant
                                              fn:FactChecker
                                            )
                              ] ;
          rdfs:subClassOf prov:Role ;
          rdfs:comment "An author of a digital document. It could be for example a Fact-Checker or a Claim Author."@en ;
          rdfs:label "Author"@en .


###  http://www.modsem.org/fakt-news#Claim
fn:Claim rdf:type owl:Class ;
         owl:equivalentClass [ owl:intersectionOf ( [ rdf:type owl:Restriction ;
                                                      owl:onProperty fn:isClaimedBy ;
                                                      owl:someValuesFrom prov:Agent
                                                    ]
                                                    [ rdf:type owl:Restriction ;
                                                      owl:onProperty fn:wasOutputOfSelection ;
                                                      owl:allValuesFrom fn:SelectionActivity
                                                    ]
                                                  ) ;
                               rdf:type owl:Class
                             ] ;
         rdfs:subClassOf fn:DigitalDocument ;
         rdfs:comment "A statement by an entity about some fact."@en ;
         rdfs:label "Claim"@en ;
         skos:altLabel "Statement"@en .


###  http://www.modsem.org/fakt-news#ClaimEvaluationActivity
fn:ClaimEvaluationActivity rdf:type owl:Class ;
                           rdfs:subClassOf prov:Activity ;
                           rdfs:comment "Last activity of fact checking process. In this activity fact checkers produces a piece of work, the review, about one or more claims supported by one or more piece of evidences."^^xsd:string ;
                           rdfs:label "Claim Evaluation Activity"@en .


###  http://www.modsem.org/fakt-news#Claimant
fn:Claimant rdf:type owl:Class ;
            rdfs:subClassOf prov:Role ;
            rdfs:comment "The entity who state the claim."@en ;
            rdfs:label "Claimant"@en .


###  http://www.modsem.org/fakt-news#CodeOfPrinciples
fn:CodeOfPrinciples rdf:type owl:Class ;
                    rdfs:subClassOf prov:Entity ;
                    rdfs:comment "A series of commitments organizations abide by to promote excellence in fact-checking."@en ;
                    rdfs:label "Code of Principles"@en .


###  http://www.modsem.org/fakt-news#ConfirmedFact
fn:ConfirmedFact rdf:type owl:Class ;
                 rdfs:subClassOf fn:Judgment ;
                 rdfs:comment "The claim content presents facts totally supported by evidence."@en ;
                 rdfs:label "Confirmed Fact"@en .


###  http://www.modsem.org/fakt-news#DeceptiveEditing
fn:DeceptiveEditing rdf:type owl:Class ;
                    rdfs:subClassOf fn:Judgment ;
                    rdfs:comment "The claim content presents facts that has been edited and rearranged in such way that ​likely to make the receiver believe something that is not true."@en ;
                    rdfs:label "Deceptive Editing"@en .


###  http://www.modsem.org/fakt-news#DigitalDocument
fn:DigitalDocument rdf:type owl:Class ;
                   rdfs:subClassOf prov:Entity .


###  http://www.modsem.org/fakt-news#DisprovingEvidence
fn:DisprovingEvidence rdf:type owl:Class ;
                      rdfs:subClassOf fn:Evidence ;
                      owl:disjointWith fn:SupportingEvidence ;
                      rdfs:comment "A disproving evidence on a certain claim."@en ;
                      rdfs:label "Disproving Evidence"@en .


###  http://www.modsem.org/fakt-news#Doctoring
fn:Doctoring rdf:type owl:Class ;
             rdfs:subClassOf fn:MaliciousTransfomation ;
             rdfs:comment "Altering the content of a claim adding or deleting visual, audio or textual information can deceive the receiver."@en ;
             rdfs:label "Doctoring"@en .


###  http://www.modsem.org/fakt-news#Editor
fn:Editor rdf:type owl:Class ;
          rdfs:subClassOf prov:Role ;
          rdfs:comment "The entity who manipulate the data in the Verification Activity. It could be the same entity as the Fact Checker."@en ;
          rdfs:label "Editor"@en .


###  http://www.modsem.org/fakt-news#Evidence
fn:Evidence rdf:type owl:Class ;
            rdfs:subClassOf prov:Entity ;
            owl:disjointUnionOf ( fn:DisprovingEvidence
                                  fn:SupportingEvidence
                                ) ;
            rdfs:comment "An evidence about a claim. Used in the verification stage of the fact-checking process."@en ;
            rdfs:label "Evidence"@en .


###  http://www.modsem.org/fakt-news#EvidenceSource
fn:EvidenceSource rdf:type owl:Class ;
                  owl:equivalentClass [ rdf:type owl:Restriction ;
                                        owl:onProperty fn:isSourceOfEvidence ;
                                        owl:someValuesFrom fn:Evidence
                                      ] ;
                  rdfs:subClassOf prov:Agent ;
                  rdfs:comment "The source of the facts. It could be the entity that states the fact itself or reports it."@en ;
                  rdfs:label "Evidence Source"@en .


###  http://www.modsem.org/fakt-news#Fabrication
fn:Fabrication rdf:type owl:Class ;
               rdfs:subClassOf fn:MaliciousTransfomation ;
               rdfs:comment "Using Artificial Intelligence to create high-quality content as fake language content, fake images, fake video, simulates audio and convincingly swaps out background images."@en ;
               rdfs:label "Fabrication"@en .


###  http://www.modsem.org/fakt-news#FactChecker
fn:FactChecker rdf:type owl:Class ;
               rdfs:subClassOf prov:Role ;
               rdfs:comment "The entity that produces a review of a claim given the claim itself and the evidence supporting it."@en ;
               rdfs:label "Fact Checker"@en .


###  http://www.modsem.org/fakt-news#FactCheckingAuthority
fn:FactCheckingAuthority rdf:type owl:Class ;
                         owl:equivalentClass [ rdf:type owl:Class ;
                                               owl:oneOf ( fn:A-1-IFCN
                                                           fn:A-13-DUKES-REPORTER-LAB
                                                         )
                                             ] ;
                         rdfs:subClassOf fn:Organization ;
                         rdfs:comment "The Fact Checking autority that monitors trends, formats and policy-making about fact-checking worldwide. It promotes and checks the committment of the fact checking organisations to ethical code standards."@en ;
                         rdfs:label "Fact Checking Authority"@en .


###  http://www.modsem.org/fakt-news#FactCheckingOrganization
fn:FactCheckingOrganization rdf:type owl:Class ;
                            rdfs:subClassOf fn:Organization ;
                            rdfs:comment "An organization that provides fact-checking services."@en ;
                            rdfs:label "Fact Checking Organization"@en .


###  http://www.modsem.org/fakt-news#FactCheckingProcess
fn:FactCheckingProcess rdf:type owl:Class ;
                       owl:equivalentClass [ owl:intersectionOf ( prov:Plan
                                                                  [ rdf:type owl:Restriction ;
                                                                    owl:onProperty fn:hasActivity ;
                                                                    owl:minQualifiedCardinality "1"^^xsd:nonNegativeInteger ;
                                                                    owl:onClass fn:ClaimEvaluationActivity
                                                                  ]
                                                                  [ rdf:type owl:Restriction ;
                                                                    owl:onProperty fn:hasActivity ;
                                                                    owl:minQualifiedCardinality "1"^^xsd:nonNegativeInteger ;
                                                                    owl:onClass fn:SelectionActivity
                                                                  ]
                                                                  [ rdf:type owl:Restriction ;
                                                                    owl:onProperty fn:hasActivity ;
                                                                    owl:minQualifiedCardinality "1"^^xsd:nonNegativeInteger ;
                                                                    owl:onClass fn:VerificationActivity
                                                                  ]
                                                                ) ;
                                             rdf:type owl:Class
                                           ] ;
                       rdfs:comment "The whole activities in which given a selected claim, supported or disproved by some evidence, generates a review article on the claim truthfulness."@en ;
                       rdfs:label "Fact Checking Process"@en .


###  http://www.modsem.org/fakt-news#Isolation
fn:Isolation rdf:type owl:Class ;
             rdfs:subClassOf fn:MissingContext ;
             rdfs:comment "Sharing a brief excerpt  from a longer story creates a false narrative that does not reflect the event as it occurred."@en ;
             rdfs:label "Isolation"@en .


###  http://www.modsem.org/fakt-news#Judgment
fn:Judgment rdf:type owl:Class ;
            rdfs:subClassOf prov:Entity ;
            rdfs:comment "A concise judgemental statement given by the fact checker to motivate the review rating"@en ;
            rdfs:label "Judgment"@en ;
            skos:altLabel "Justification"@en ,
                          "Reason"@en .


###  http://www.modsem.org/fakt-news#MaliciousTransfomation
fn:MaliciousTransfomation rdf:type owl:Class ;
                          rdfs:subClassOf fn:Judgment ;
                          rdfs:comment "Part or all of the claim content has been manipulated to transform the content itself."@en ;
                          rdfs:label "Malicious Transformation"@en .


###  http://www.modsem.org/fakt-news#Misrepresentation
fn:Misrepresentation rdf:type owl:Class ;
                     rdfs:subClassOf fn:MissingContext ;
                     rdfs:comment "Presenting unaltered content in an inaccurate manner misrepresents the content itself and misleads the receiver"@en ;
                     rdfs:label "Misrepresentation"@en .


###  http://www.modsem.org/fakt-news#MissingContext
fn:MissingContext rdf:type owl:Class ;
                  rdfs:subClassOf fn:Judgment ;
                  rdfs:comment "The claim content lacks or misstates the context in which events occurred."@en ;
                  rdfs:label "Missing Context"@en .


###  http://www.modsem.org/fakt-news#NotClearGeographyContext
fn:NotClearGeographyContext rdf:type owl:Class ;
                            rdfs:subClassOf fn:Misrepresentation ;
                            rdfs:comment "The geographic context is incorrect or not clear such as event incorrect location."@en ;
                            rdfs:label "Not Clear Geography Context"@en ;
                            skos:altLabel "Misrepresented Geography Context"@en .


###  http://www.modsem.org/fakt-news#NotClearPeriodContext
fn:NotClearPeriodContext rdf:type owl:Class ;
                         rdfs:subClassOf fn:Misrepresentation ;
                         rdfs:comment "The time context is incorrect or not clear such as event incorrect date."@en ;
                         rdfs:label "Not Clear Time Period Context"@en ;
                         skos:altLabel "Misrepresented Time Period Context"@en .


###  http://www.modsem.org/fakt-news#NotClearSubject
fn:NotClearSubject rdf:type owl:Class ;
                   rdfs:subClassOf fn:Misrepresentation ;
                   rdfs:comment "The subject entity of the claim is incorrect or not clear."@en ;
                   rdfs:label "Not Clear Subject"@en ;
                   skos:altLabel "Misrepresented Subject"@en .


###  http://www.modsem.org/fakt-news#Omission
fn:Omission rdf:type owl:Class ;
            rdfs:subClassOf fn:DeceptiveEditing ;
            rdfs:comment "Editing out large portions from a video and presenting it as a complete narrative, despite missing key elements, produce a skew reality."@en ;
            rdfs:label "Omission"@en .


###  http://www.modsem.org/fakt-news#Organization
fn:Organization rdf:type owl:Class ;
                rdfs:subClassOf prov:Agent ;
                rdfs:comment "A group of persons grouped together or organized for some purpose or work."@en ;
                rdfs:label "Organization"@en .


###  http://www.modsem.org/fakt-news#Person
fn:Person rdf:type owl:Class ;
          owl:equivalentClass foaf:Person ;
          rdfs:subClassOf prov:Agent ;
          rdfs:comment "A real human person."@en ;
          rdfs:label "Person"@en .


###  http://www.modsem.org/fakt-news#QualitativeClaim
fn:QualitativeClaim rdf:type owl:Class ;
                    rdfs:subClassOf fn:Judgment ;
                    rdfs:comment "The claim use qualitative information in place of quantitative descriptions that are open to the receiver interpretation."^^xsd:string ;
                    rdfs:label "Qualitative Claim"@en ;
                    skos:example "\"... in my past five years as leader, I have increased employment.\" is a qualitative claim. This could corresponds to a quantitive information as \"In the past five years, employment has risen from 95.0% to 95.05%.\""^^xsd:string .


###  http://www.modsem.org/fakt-news#Rating
fn:Rating rdf:type owl:Class ;
          rdfs:subClassOf prov:Entity ;
          rdfs:comment "A rating of a review within a known evaluation meter. The rating value can belong to an external rating system."@en ;
          rdfs:label "Rating"@en .


###  http://www.modsem.org/fakt-news#Review
fn:Review rdf:type owl:Class ;
          owl:equivalentClass [ owl:intersectionOf ( [ rdf:type owl:Restriction ;
                                                       owl:onProperty fn:isReviewedBy ;
                                                       owl:someValuesFrom prov:Agent
                                                     ]
                                                     [ rdf:type owl:Restriction ;
                                                       owl:onProperty fn:wasOutputOfClaimEvaluation ;
                                                       owl:allValuesFrom fn:ClaimEvaluationActivity
                                                     ]
                                                   ) ;
                                rdf:type owl:Class
                              ] ;
          rdfs:subClassOf fn:DigitalDocument ;
          rdfs:comment "The final document that contains the review of a claim by a fact-checker."^^xsd:string ;
          rdfs:label "Review"@en .


###  http://www.modsem.org/fakt-news#SelectionActivity
fn:SelectionActivity rdf:type owl:Class ;
                     rdfs:subClassOf prov:Activity ;
                     rdfs:comment "First activity of fact checking process. In this activity fact checkers select one or more claims from a list of suggested alternatives guided by the selection policy."@en ;
                     rdfs:label "Selection Activity"@en .


###  http://www.modsem.org/fakt-news#SoftwareAgent
fn:SoftwareAgent rdf:type owl:Class ;
                 rdfs:subClassOf prov:Agent ;
                 rdfs:comment "A software program that act in automounus way in some kind of environment to achive some kind of task."@en ;
                 rdfs:label "Software Agent"@en ;
                 skos:altLabel "Bot, Software"@en .


###  http://www.modsem.org/fakt-news#Splicing
fn:Splicing rdf:type owl:Class ;
            rdfs:subClassOf fn:DeceptiveEditing ;
            rdfs:comment "Editing together different excerpts fundamentally alters the story that is being told. An example is glueing together quotes without context."@en ;
            rdfs:label "Splicing"@en .


###  http://www.modsem.org/fakt-news#SupportingEvidence
fn:SupportingEvidence rdf:type owl:Class ;
                      rdfs:subClassOf fn:Evidence ;
                      rdfs:comment "A proving evidence on a certain claim."@en ;
                      rdfs:label "Supporting Evidence"@en .


###  http://www.modsem.org/fakt-news#TrustedSource
fn:TrustedSource rdf:type owl:Class ;
                 owl:equivalentClass [ rdf:type owl:Class ;
                                       owl:unionOf ( [ rdf:type owl:Restriction ;
                                                       owl:onProperty fn:capacityType ;
                                                       owl:hasValue "Government"
                                                     ]
                                                     [ rdf:type owl:Restriction ;
                                                       owl:onProperty fn:capacityType ;
                                                       owl:hasValue "NGO"
                                                     ]
                                                     [ rdf:type owl:Restriction ;
                                                       owl:onProperty fn:capacityType ;
                                                       owl:hasValue "Think Tank"
                                                     ]
                                                   )
                                     ] ;
                 rdfs:subClassOf fn:EvidenceSource ;
                 rdfs:comment "A Trusted Source is known to be reliable because its authority or authenticity is widely recognized by experts in the field."@en ;
                 rdfs:label "Trusted Source"@en ;
                 skos:altLabel "Authoritative Source"@en .


###  http://www.modsem.org/fakt-news#VerificationActivity
fn:VerificationActivity rdf:type owl:Class ;
                        rdfs:subClassOf prov:Activity ;
                        rdfs:comment "In this activity fact checkers searches piece of evidences to verify the validity of a given claim"@en ;
                        rdfs:label "Verification Activity"@en .


###  http://www.ontologydesignpatterns.org/cp/owl/collectionentity.owl#Collection
<http://www.ontologydesignpatterns.org/cp/owl/collectionentity.owl#Collection> rdfs:subClassOf prov:Entity .


###  http://www.ontologydesignpatterns.org/cp/owl/timeinterval.owl#TimeInterval
<http://www.ontologydesignpatterns.org/cp/owl/timeinterval.owl#TimeInterval> rdfs:subClassOf prov:Entity .


###  http://www.w3.org/ns/prov#Activity
prov:Activity rdf:type owl:Class ;
              rdfs:comment "An activity is something that occurs over a period of time and acts upon or with entities; it may include consuming, processing, transforming, modifying, relocating, using, or generating entities."@en ;
              rdfs:label "Activity"@en .


###  http://www.w3.org/ns/prov#Agent
prov:Agent rdf:type owl:Class ;
           rdfs:comment "An agent is something that bears some form of responsibility for an activity taking place, for the existence of an entity, or for another agent's activity."@en ;
           rdfs:label "Agent"@en .


###  http://www.w3.org/ns/prov#Association
prov:Association rdf:type owl:Class ;
                 rdfs:comment "An activity association is an assignment of responsibility to an agent for an activity, indicating that the agent had a role in the activity. It further allows for a plan to be specified, which is the plan intended by the agent to achieve some goals in the context of this activity."@en ;
                 rdfs:label "Association"@en .


###  http://www.w3.org/ns/prov#Entity
prov:Entity rdf:type owl:Class ;
            rdfs:comment "An entity is a physical, digital, conceptual, or other kind of thing with some fixed aspects; entities may be real or imaginary."@en ;
            rdfs:label "Entity"@en .


###  http://www.w3.org/ns/prov#Plan
prov:Plan rdf:type owl:Class ;
          rdfs:subClassOf prov:Entity ;
          rdfs:comment "A plan is an entity that represents a set of actions or steps intended by one or more agents to achieve some goals."@en ;
          rdfs:label "Plan"@en .


###  http://www.w3.org/ns/prov#Role
prov:Role rdf:type owl:Class ;
          rdfs:comment "A role is the function of an entity or agent with respect to an activity, in the context of a usage, generation, invalidation, association, start, and end."@en ;
          rdfs:label "Role"@en .


###  http://xmlns.com/foaf/0.1/Person
foaf:Person rdf:type owl:Class ;
            rdfs:subClassOf prov:Agent ;
            rdfs:comment "The Person class represents people. Something is a Person if it is a person. We don't nitpic about whether they're alive, dead, real, or imaginary. The Person class is a sub-class of the Agent class, since all people are considered 'agents' in FOAF."@en ;
            rdfs:label "Person"@en .


#################################################################
#    Individuals
#################################################################

###  http://www.modsem.org/fakt-news#A-1-IFCN
fn:A-1-IFCN rdf:type owl:NamedIndividual ,
                     fn:Organization ;
            fn:create fn:IFCN-Code-of-Principles ;
            fn:createCodeOfPrinciples fn:IFCN-Code-of-Principles ;
            schema:name "International Fact Checking Organization"^^xsd:string ;
            schema:url "https://www.poynter.org/ifcn/"^^xsd:anyURI .


###  http://www.modsem.org/fakt-news#A-10
fn:A-10 rdf:type owl:NamedIndividual ,
                 fn:Person ,
                 prov:Agent ,
                 foaf:Person ;
        fn:create fn:C-2 ;
        schema:name "Matteo Salvini"^^xsd:string .


###  http://www.modsem.org/fakt-news#A-11
fn:A-11 rdf:type owl:NamedIndividual ,
                 fn:Person ,
                 prov:Agent ,
                 foaf:Person ;
        fn:create fn:C-3 ;
        schema:name "Mark Zucherberg"^^xsd:string .


###  http://www.modsem.org/fakt-news#A-12
fn:A-12 rdf:type owl:NamedIndividual ,
                 fn:Person ,
                 prov:Agent ,
                 foaf:Person ;
        fn:create fn:C-4 ;
        schema:name "America Divided Podcast"^^xsd:string .


###  http://www.modsem.org/fakt-news#A-13-DUKES-REPORTER-LAB
fn:A-13-DUKES-REPORTER-LAB rdf:type owl:NamedIndividual ,
                                    fn:Organization ;
                           schema:name "Duke Reporter's Lab"^^xsd:string ;
                           schema:url "https://reporterslab.org/"^^xsd:anyURI .


###  http://www.modsem.org/fakt-news#A-14
fn:A-14 rdf:type owl:NamedIndividual ,
                 fn:Person ,
                 prov:Agent ,
                 foaf:Person ;
        schema:name "Tommaso Canetta"^^xsd:string .


###  http://www.modsem.org/fakt-news#A-2
fn:A-2 rdf:type owl:NamedIndividual ,
                fn:FactCheckingOrganization ,
                fn:Organization ,
                prov:Agent ;
       fn:observeCodeOfPrinciples fn:IFCN-Code-of-Principles ;
       schema:name "Lavoce.info"^^xsd:string .


###  http://www.modsem.org/fakt-news#A-3
fn:A-3 rdf:type owl:NamedIndividual ,
                fn:Person ,
                prov:Agent ,
                foaf:Person ;
       fn:affiliatedTo fn:A-2 ;
       fn:create fn:R-1 ;
       schema:name "Massimo Taddei"^^xsd:string .


###  http://www.modsem.org/fakt-news#A-4
fn:A-4 rdf:type owl:NamedIndividual ,
                fn:FactCheckingOrganization ,
                fn:Organization ,
                prov:Agent ;
       fn:create fn:R-2 ;
       fn:observeCodeOfPrinciples fn:IFCN-Code-of-Principles ;
       schema:name "Pagella Politica"^^xsd:string .


###  http://www.modsem.org/fakt-news#A-5
fn:A-5 rdf:type owl:NamedIndividual ,
                fn:Organization ,
                prov:Agent ;
       schema:name "Washington Post"^^xsd:string .


###  http://www.modsem.org/fakt-news#A-6
fn:A-6 rdf:type owl:NamedIndividual ,
                fn:Person ,
                prov:Agent ,
                foaf:Person ;
       fn:affiliatedTo fn:A-5 ;
       fn:create fn:R-3 ;
       schema:name "Allyson Chiu"^^xsd:string .


###  http://www.modsem.org/fakt-news#A-7
fn:A-7 rdf:type owl:NamedIndividual ,
                fn:FactCheckingOrganization ,
                fn:Organization ,
                prov:Agent ;
       fn:observeCodeOfPrinciples fn:IFCN-Code-of-Principles ;
       schema:name "Politifact.com"^^xsd:string .


###  http://www.modsem.org/fakt-news#A-8
fn:A-8 rdf:type owl:NamedIndividual ,
                fn:Person ,
                prov:Agent ,
                foaf:Person ;
       fn:affiliatedTo fn:A-7 ;
       fn:create fn:R-4 ;
       schema:name "Daniel Funke"^^xsd:string .


###  http://www.modsem.org/fakt-news#A-9
fn:A-9 rdf:type owl:NamedIndividual ,
                fn:Person ,
                prov:Agent ,
                foaf:Person ;
       fn:create fn:C-1 ;
       schema:name "Nicola Zingaretti"^^xsd:string .


###  http://www.modsem.org/fakt-news#Activity-Evaluation-R-1
fn:Activity-Evaluation-R-1 rdf:type owl:NamedIndividual ,
                                    fn:ClaimEvaluationActivity ,
                                    prov:Activity ;
                           fn:hasPreviousActivity fn:Activity-Verification-R-1 ;
                           fn:hasTimeInterval fn:Time-R1-2020-10-07-2020-10-08 ;
                           fn:isActivityOfPlan fn:Plan-R-1 ;
                           fn:isLastActivityOfPlan fn:Plan-R-1 ;
                           fn:isUsedByClaimEvaluation fn:Evidence-R-1 ;
                           prov:qualifiedAssociation fn:Association-Activity-Evaluation-R1-A3 ;
                           prov:used fn:Evidence-R-1 .


###  http://www.modsem.org/fakt-news#Activity-Evaluation-R-2
fn:Activity-Evaluation-R-2 rdf:type owl:NamedIndividual ,
                                    fn:ClaimEvaluationActivity ,
                                    prov:Activity ;
                           fn:hasPreviousActivity fn:Activity-Verification-R-2 ;
                           fn:hasTimeInterval fn:Time-R2-2021-01-15-2021-01-16 ;
                           fn:isActivityOfPlan fn:Plan-R-2 ;
                           fn:isLastActivityOfPlan fn:Plan-R-2 ;
                           fn:isUsedByClaimEvaluation fn:Evidence-R-2 ;
                           prov:qualifiedAssociation fn:Association-Activity-Evaluation-R2-A4 ;
                           prov:used fn:Evidence-R-2 .


###  http://www.modsem.org/fakt-news#Activity-Evaluation-R-3
fn:Activity-Evaluation-R-3 rdf:type owl:NamedIndividual ,
                                    fn:ClaimEvaluationActivity ,
                                    prov:Activity ;
                           fn:hasPreviousActivity fn:Activity-Verification-R-3 ;
                           fn:hasTimeInterval fn:Time-R3-2019-06-18-2019-06-19 ;
                           fn:isActivityOfPlan fn:Plan-R-3 ;
                           fn:isLastActivityOfPlan fn:Plan-R-3 ;
                           fn:isUsedByClaimEvaluation fn:Evidence-R-3 ;
                           prov:qualifiedAssociation fn:Association-Activity-Evaluation-R3-A6 ;
                           prov:used fn:Evidence-R-3 .


###  http://www.modsem.org/fakt-news#Activity-Evaluation-R-4
fn:Activity-Evaluation-R-4 rdf:type owl:NamedIndividual ,
                                    fn:ClaimEvaluationActivity ,
                                    prov:Activity ;
                           fn:hasPreviousActivity fn:Activity-Verification-R-4 ;
                           fn:hasTimeInterval fn:Time-R4-2021-01-19-2021-01-20 ;
                           fn:isActivityOfPlan fn:Plan-R-4 ;
                           fn:isLastActivityOfPlan fn:Plan-R-4 ;
                           fn:isUsedByClaimEvaluation fn:Evidence-R-4 ;
                           prov:qualifiedAssociation fn:Association-Activity-Evaluation-R4-A8 ;
                           prov:used fn:Evidence-R-4 .


###  http://www.modsem.org/fakt-news#Activity-Selection-R-1
fn:Activity-Selection-R-1 rdf:type owl:NamedIndividual ,
                                   fn:SelectionActivity ,
                                   prov:Activity ;
                          fn:hasNextActivity fn:Activity-Verification-R-1 ;
                          fn:hasTimeInterval fn:Time-R1-2020-10-05-2020-10-06 ;
                          fn:isActivityOfPlan fn:Plan-R-1 ;
                          fn:isFirstActivityOfPlan fn:Plan-R-1 ;
                          fn:isUsedBySelection fn:Alternative-Set-R-1 ;
                          prov:qualifiedAssociation fn:Association-Activity-Selection-R1-A9 ;
                          prov:used fn:Alternative-Set-R-1 .


###  http://www.modsem.org/fakt-news#Activity-Selection-R-2
fn:Activity-Selection-R-2 rdf:type owl:NamedIndividual ,
                                   fn:SelectionActivity ,
                                   prov:Activity ;
                          fn:hasNextActivity fn:Activity-Verification-R-2 ;
                          fn:hasTimeInterval fn:Time-R2-2021-01-13-2021-01-14 ;
                          fn:isActivityOfPlan fn:Plan-R-2 ;
                          fn:isFirstActivityOfPlan fn:Plan-R-2 ;
                          prov:qualifiedAssociation fn:Association-Activity-Selection-R2-A10 ,
                                                    fn:Association-Activity-Selection-R2-A14 .


###  http://www.modsem.org/fakt-news#Activity-Selection-R-3
fn:Activity-Selection-R-3 rdf:type owl:NamedIndividual ,
                                   fn:SelectionActivity ,
                                   prov:Activity ;
                          fn:hasNextActivity fn:Activity-Verification-R-3 ;
                          fn:hasTimeInterval fn:Time-R3-2019-06-16-2019-06-17 ;
                          fn:isActivityOfPlan fn:Plan-R-3 ;
                          fn:isFirstActivityOfPlan fn:Plan-R-3 ;
                          prov:qualifiedAssociation fn:Association-Activity-Selection-R3-A11 .


###  http://www.modsem.org/fakt-news#Activity-Selection-R-4
fn:Activity-Selection-R-4 rdf:type owl:NamedIndividual ,
                                   fn:SelectionActivity ,
                                   prov:Activity ;
                          fn:hasNextActivity fn:Activity-Verification-R-4 ;
                          fn:hasTimeInterval fn:Time-R4-2021-01-17-2021-01-18 ;
                          fn:isActivityOfPlan fn:Plan-R-4 ;
                          fn:isFirstActivityOfPlan fn:Plan-R-4 ;
                          prov:qualifiedAssociation fn:Association-Activity-Selection-R4-A12 .


###  http://www.modsem.org/fakt-news#Activity-Verification-R-1
fn:Activity-Verification-R-1 rdf:type owl:NamedIndividual ,
                                      fn:VerificationActivity ,
                                      prov:Activity ;
                             fn:hasNextActivity fn:Activity-Evaluation-R-1 ;
                             fn:hasPreviousActivity fn:Activity-Selection-R-1 ;
                             fn:hasTimeInterval fn:Time-R1-2020-10-06-2020-10-07 ;
                             fn:isActivityOfPlan fn:Plan-R-1 ;
                             fn:isUsedByVerification fn:C-1 ;
                             prov:used fn:C-1 .


###  http://www.modsem.org/fakt-news#Activity-Verification-R-2
fn:Activity-Verification-R-2 rdf:type owl:NamedIndividual ,
                                      fn:VerificationActivity ,
                                      prov:Activity ;
                             fn:hasNextActivity fn:Activity-Evaluation-R-2 ;
                             fn:hasPreviousActivity fn:Activity-Selection-R-2 ;
                             fn:hasTimeInterval fn:Time-R2-2021-01-14-2021-01-15 ;
                             fn:isActivityOfPlan fn:Plan-R-2 ;
                             fn:isUsedByVerification fn:C-2 ;
                             prov:used fn:C-2 .


###  http://www.modsem.org/fakt-news#Activity-Verification-R-3
fn:Activity-Verification-R-3 rdf:type owl:NamedIndividual ,
                                      fn:VerificationActivity ,
                                      prov:Activity ;
                             fn:hasNextActivity fn:Activity-Evaluation-R-3 ;
                             fn:hasPreviousActivity fn:Activity-Selection-R-3 ;
                             fn:hasTimeInterval fn:Time-R3-2019-06-17-2019-06-18 ;
                             fn:isActivityOfPlan fn:Plan-R-3 ;
                             fn:isUsedByVerification fn:C-3 ;
                             prov:used fn:C-3 .


###  http://www.modsem.org/fakt-news#Activity-Verification-R-4
fn:Activity-Verification-R-4 rdf:type owl:NamedIndividual ,
                                      fn:VerificationActivity ,
                                      prov:Activity ;
                             fn:hasNextActivity fn:Activity-Evaluation-R-4 ;
                             fn:hasPreviousActivity fn:Activity-Selection-R-4 ;
                             fn:hasTimeInterval fn:Time-R4-2021-01-18-2021-01-19 ;
                             fn:isActivityOfPlan fn:Plan-R-4 ;
                             fn:isUsedByVerification fn:C-4 ;
                             prov:used fn:C-4 .


###  http://www.modsem.org/fakt-news#Alternative-Set-R-1
fn:Alternative-Set-R-1 rdf:type owl:NamedIndividual ,
                                fn:AlternativesSet ,
                                <http://www.ontologydesignpatterns.org/cp/owl/collectionentity.owl#Collection> ,
                                <http://www.ontologydesignpatterns.org/cp/owl/set.owl#Set> ,
                                prov:Entity ;
                       <http://www.ontologydesignpatterns.org/cp/owl/collectionentity.owl#hasMember> fn:C-1 ,
                                                                                                     fn:C-2 .


###  http://www.modsem.org/fakt-news#Association-Activity-Evaluation-R1-A3
fn:Association-Activity-Evaluation-R1-A3 rdf:type owl:NamedIndividual ,
                                                  prov:Association ;
                                         prov:agent fn:A-3 ;
                                         prov:hadRole fn:Role-A-3 .


###  http://www.modsem.org/fakt-news#Association-Activity-Evaluation-R2-A4
fn:Association-Activity-Evaluation-R2-A4 rdf:type owl:NamedIndividual ,
                                                  prov:Association ;
                                         prov:agent fn:A-4 ;
                                         prov:hadRole fn:Role-A-4 .


###  http://www.modsem.org/fakt-news#Association-Activity-Evaluation-R3-A6
fn:Association-Activity-Evaluation-R3-A6 rdf:type owl:NamedIndividual ,
                                                  prov:Association ;
                                         prov:agent fn:A-6 ;
                                         prov:hadRole fn:Role-A-6 .


###  http://www.modsem.org/fakt-news#Association-Activity-Evaluation-R4-A8
fn:Association-Activity-Evaluation-R4-A8 rdf:type owl:NamedIndividual ,
                                                  prov:Association ;
                                         prov:agent fn:A-8 ;
                                         prov:hadRole fn:Role-A-8 .


###  http://www.modsem.org/fakt-news#Association-Activity-Selection-R1-A9
fn:Association-Activity-Selection-R1-A9 rdf:type owl:NamedIndividual ,
                                                 prov:Association ;
                                        prov:agent fn:A-9 ;
                                        prov:hadRole fn:Role-A-9 .


###  http://www.modsem.org/fakt-news#Association-Activity-Selection-R2-A10
fn:Association-Activity-Selection-R2-A10 rdf:type owl:NamedIndividual ,
                                                  prov:Association ;
                                         prov:agent fn:A-10 ;
                                         prov:hadRole fn:Role-A-10 .


###  http://www.modsem.org/fakt-news#Association-Activity-Selection-R2-A14
fn:Association-Activity-Selection-R2-A14 rdf:type owl:NamedIndividual ,
                                                  prov:Association ;
                                         prov:agent fn:A-14 ;
                                         prov:hadRole fn:Role-A-14 .


###  http://www.modsem.org/fakt-news#Association-Activity-Selection-R3-A11
fn:Association-Activity-Selection-R3-A11 rdf:type owl:NamedIndividual ,
                                                  prov:Association ;
                                         prov:agent fn:A-11 ;
                                         prov:hadRole fn:Role-A-11 .


###  http://www.modsem.org/fakt-news#Association-Activity-Selection-R4-A12
fn:Association-Activity-Selection-R4-A12 rdf:type owl:NamedIndividual ,
                                                  prov:Association ;
                                         prov:agent fn:A-12 ;
                                         prov:hadRole fn:Role-A-12 .


###  http://www.modsem.org/fakt-news#C-1
fn:C-1 rdf:type owl:NamedIndividual ,
                schema:CreativeWork ,
                fn:Claim ,
                fn:DigitalDocument ,
                prov:Entity ;
       fn:associatedReview fn:R-1 ;
       fn:creator fn:A-9 ;
       fn:isClaimedBy fn:A-9 ;
       fn:wasOutputOfSelection fn:Activity-Selection-R-1 ;
       prov:wasAttributedTo fn:A-9 ;
       prov:wasGeneratedBy fn:Activity-Selection-R-1 ;
       dcterms:date "2020-10-05"^^xsd:date ;
       dcterms:language "it"^^xsd:string ;
       schema:url "https://twitter.com/nzingaretti/status/1313218301200400389?ref_src=twsrc%5Etfw"^^xsd:anyURI ;
       fn:claimContent "Approvato ora in Consiglio dei Ministri il decreto immigrazione. I decreti propaganda/Salvini non ci sono più. Vogliamo un’Italia  più umana e sicura. Un’Europa più protagonista"^^xsd:string ;
       fn:documentContent "Approvato ora in Consiglio dei Ministri il decreto immigrazione. I decreti propaganda/Salvini non ci sono più. Vogliamo un’Italia  più umana e sicura. Un’Europa più protagonista"^^xsd:string ;
       <http://www.ontologydesignpatterns.org/cp/owl/collectionentity.owl#isMemberOf> fn:Alternative-Set-R-1 .


###  http://www.modsem.org/fakt-news#C-2
fn:C-2 rdf:type owl:NamedIndividual ,
                schema:CreativeWork ,
                fn:Claim ,
                fn:DigitalDocument ,
                prov:Entity ;
       fn:associatedReview fn:R-2 ;
       fn:creator fn:A-10 ;
       fn:isClaimedBy fn:A-10 ;
       prov:wasAttributedTo fn:A-10 ;
       dcterms:date "2021-01-13"^^xsd:date ;
       dcterms:language "it"^^xsd:string ;
       schema:url "https://twitter.com/matteosalvinimi/status/1349377644941479937"^^xsd:anyURI ;
       fn:claimContent "Con tutti i problemi che ci sono in Italia, al governo si preoccupano di cancellare “padre” e “madre” dalla carta di identità dei minori per sostituirli con Genitore 1 e 2. Prima vanno a casa, meglio è."^^xsd:string ;
       fn:documentContent "Con tutti i problemi che ci sono in Italia, al governo si preoccupano di cancellare “padre” e “madre” dalla carta di identità dei minori per sostituirli con Genitore 1 e 2. Prima vanno a casa, meglio è."^^xsd:string ;
       <http://www.ontologydesignpatterns.org/cp/owl/collectionentity.owl#isMemberOf> fn:Alternative-Set-R-1 .


###  http://www.modsem.org/fakt-news#C-3
fn:C-3 rdf:type owl:NamedIndividual ,
                schema:CreativeWork ,
                fn:Claim ,
                fn:DigitalDocument ,
                prov:Entity ;
       fn:associatedReview fn:R-3 ;
       fn:creator fn:A-11 ;
       fn:isClaimedBy fn:A-11 ;
       prov:wasAttributedTo fn:A-11 ;
       dcterms:date "2019-06-07"^^xsd:date ;
       dcterms:language "en"^^xsd:string ;
       schema:url "https://www.instagram.com/p/ByaVigGFP2U/?utm_source=ig_embed&utm_campaign=embed_video_watch_again"^^xsd:anyURI ;
       fn:claimContent "Zuckerberg: we are increasing transparency on Ads. Announces new measure to protect the elections."^^xsd:string ;
       fn:documentContent "Zuckerberg: we are increasing transparency on Ads. Announces new measure to protect the elections."^^xsd:string .


###  http://www.modsem.org/fakt-news#C-4
fn:C-4 rdf:type owl:NamedIndividual ,
                schema:CreativeWork ,
                fn:Claim ,
                fn:DigitalDocument ,
                prov:Entity ;
       fn:associatedReview fn:R-4 ;
       fn:creator fn:A-12 ;
       fn:isClaimedBy fn:A-12 ;
       prov:wasAttributedTo fn:A-12 ;
       dcterms:date "2021-01-17"^^xsd:date ;
       dcterms:language "en"^^xsd:string ;
       schema:url "https://archive.vn/5P96s"^^xsd:anyURI ;
       fn:claimContent "Barack Obama was arrested: a video published on Facebook claims to show former President Barack Obama in jail."^^xsd:string ;
       fn:documentContent "Barack Obama was arrested: a video published on Facebook claims to show former President Barack Obama in jail."^^xsd:string .


###  http://www.modsem.org/fakt-news#Evidence-Document-R-1
fn:Evidence-Document-R-1 rdf:type owl:NamedIndividual ,
                                  schema:CreativeWork ,
                                  fn:DigitalDocument ,
                                  prov:Entity ;
                         dcterms:language "it"^^xsd:string ;
                         schema:url "http://www.cir-onlus.org/wp-content/uploads/2018/11/Speciale-Decreto-Sicurezza.pdf"^^xsd:anyURI .


###  http://www.modsem.org/fakt-news#Evidence-Document-R-2
fn:Evidence-Document-R-2 rdf:type owl:NamedIndividual ,
                                  schema:CreativeWork ,
                                  fn:DigitalDocument ,
                                  prov:Entity ;
                         dcterms:language "it"^^xsd:string ;
                         schema:url "https://www.gazzettaufficiale.it/eli/gu/2015/08/14/188/so/49/sg/pdf#page=99"^^xsd:anyURI .


###  http://www.modsem.org/fakt-news#Evidence-Document-R-3
fn:Evidence-Document-R-3 rdf:type owl:NamedIndividual ,
                                  schema:CreativeWork ,
                                  fn:DigitalDocument ,
                                  prov:Entity ;
                         dcterms:language "en"^^xsd:string ;
                         schema:url "https://www.instagram.com/p/CBOIEh3lhPr/"^^xsd:anyURI .


###  http://www.modsem.org/fakt-news#Evidence-Document-R-4
fn:Evidence-Document-R-4 rdf:type owl:NamedIndividual ,
                                  schema:CreativeWork ,
                                  fn:DigitalDocument ,
                                  prov:Entity ;
                         dcterms:language "en"^^xsd:string ;
                         schema:url "https://www.youtube.com/watch?v=fGZTFg8PP9Q&feature=youtu.be"^^xsd:anyURI .


###  http://www.modsem.org/fakt-news#Evidence-Document2-R-4
fn:Evidence-Document2-R-4 rdf:type owl:NamedIndividual ,
                                   schema:CreativeWork ,
                                   fn:DigitalDocument ,
                                   prov:Entity ;
                          dcterms:language "en"^^xsd:string ;
                          schema:url "https://obamawhitehouse.archives.gov/blog/2013/06/30/flotus-travel-journal-robben-island-experience-we-will-never-forget"^^xsd:anyURI .


###  http://www.modsem.org/fakt-news#Evidence-R-1
fn:Evidence-R-1 rdf:type owl:NamedIndividual ,
                         fn:Evidence ,
                         fn:SupportingEvidence ,
                         prov:Entity ;
                fn:derivedFromSource fn:EvidenceSource-R-1 ;
                fn:supportedBy fn:Evidence-Document-R-1 ;
                fn:wasOutputOfVerification fn:Activity-Verification-R-1 ;
                prov:wasAttributedTo fn:EvidenceSource-R-1 ;
                prov:wasGeneratedBy fn:Activity-Verification-R-1 .


###  http://www.modsem.org/fakt-news#Evidence-R-2
fn:Evidence-R-2 rdf:type owl:NamedIndividual ,
                         fn:DisprovingEvidence ,
                         fn:Evidence ,
                         prov:Entity ;
                fn:derivedFromSource fn:EvidenceSource-R-2 ;
                fn:supportedBy fn:Evidence-Document-R-2 ;
                fn:wasOutputOfVerification fn:Activity-Verification-R-2 ;
                prov:wasAttributedTo fn:EvidenceSource-R-2 ;
                prov:wasGeneratedBy fn:Activity-Verification-R-2 .


###  http://www.modsem.org/fakt-news#Evidence-R-3
fn:Evidence-R-3 rdf:type owl:NamedIndividual ,
                         fn:DisprovingEvidence ,
                         fn:Evidence ,
                         prov:Entity ;
                fn:derivedFromSource fn:EvidenceSource-R-3 ;
                fn:supportedBy fn:Evidence-Document-R-3 ;
                fn:wasOutputOfVerification fn:Activity-Verification-R-3 ;
                prov:wasAttributedTo fn:EvidenceSource-R-3 ;
                prov:wasGeneratedBy fn:Activity-Verification-R-3 .


###  http://www.modsem.org/fakt-news#Evidence-R-4
fn:Evidence-R-4 rdf:type owl:NamedIndividual ,
                         fn:DisprovingEvidence ,
                         fn:Evidence ,
                         prov:Entity ;
                fn:derivedFromSource fn:EvidenceSource-R-4 ;
                fn:supportedBy fn:Evidence-Document-R-4 ;
                fn:wasOutputOfVerification fn:Activity-Verification-R-4 ;
                prov:wasAttributedTo fn:EvidenceSource-R-4 ;
                prov:wasGeneratedBy fn:Activity-Verification-R-4 .


###  http://www.modsem.org/fakt-news#Evidence2-R-4
fn:Evidence2-R-4 rdf:type owl:NamedIndividual ,
                          fn:DisprovingEvidence ,
                          fn:Evidence ,
                          prov:Entity ;
                 fn:derivedFromSource fn:EvidenceSource2-R-4 ;
                 fn:supportedBy fn:Evidence-Document2-R-4 ;
                 fn:wasOutputOfVerification fn:Activity-Verification-R-4 ;
                 prov:wasAttributedTo fn:EvidenceSource2-R-4 ;
                 prov:wasGeneratedBy fn:Activity-Verification-R-4 .


###  http://www.modsem.org/fakt-news#EvidenceSource-R-1
fn:EvidenceSource-R-1 rdf:type owl:NamedIndividual ,
                               fn:EvidenceSource ,
                               fn:Organization ,
                               prov:Agent ;
                      fn:isSourceOfEvidence fn:Evidence-R-1 ;
                      schema:name "Consiglio Italiano per i Rifugiati (CIR)"^^xsd:string ;
                      schema:url "http://www.cir-onlus.org/"^^xsd:anyURI ;
                      fn:capacityType "NGO"^^xsd:string .


###  http://www.modsem.org/fakt-news#EvidenceSource-R-2
fn:EvidenceSource-R-2 rdf:type owl:NamedIndividual ,
                               fn:EvidenceSource ,
                               fn:Organization ,
                               prov:Agent ;
                      fn:isSourceOfEvidence fn:Evidence-R-2 ;
                      schema:name "Governo Italiano"^^xsd:string ;
                      schema:url "http://www.governo.it/"^^xsd:anyURI ;
                      fn:capacityType "Government"^^xsd:string .


###  http://www.modsem.org/fakt-news#EvidenceSource-R-3
fn:EvidenceSource-R-3 rdf:type owl:NamedIndividual ,
                               fn:EvidenceSource ,
                               fn:Person ,
                               prov:Agent ,
                               foaf:Person ;
                      fn:isSourceOfEvidence fn:Evidence-R-3 ;
                      schema:name "Bill Posters"^^xsd:string ;
                      schema:url "https://www.instagram.com/bill_posters_uk/"^^xsd:anyURI ;
                      fn:capacityType "Citizen"^^xsd:string .


###  http://www.modsem.org/fakt-news#EvidenceSource-R-4
fn:EvidenceSource-R-4 rdf:type owl:NamedIndividual ,
                               fn:EvidenceSource ,
                               fn:Organization ,
                               prov:Agent ;
                      fn:isSourceOfEvidence fn:Evidence-R-4 ;
                      schema:name "The Guardian"^^xsd:string ;
                      schema:url "https://www.theguardian.com/international"^^xsd:anyURI ;
                      fn:capacityType "Company"^^xsd:string .


###  http://www.modsem.org/fakt-news#EvidenceSource2-R-4
fn:EvidenceSource2-R-4 rdf:type owl:NamedIndividual ,
                                fn:EvidenceSource ,
                                fn:Organization ,
                                prov:Agent ;
                       fn:isSourceOfEvidence fn:Evidence2-R-4 ;
                       schema:name "The White House"^^xsd:string ;
                       schema:url "https://www.whitehouse.gov"^^xsd:anyURI ;
                       fn:capacityType "Government"^^xsd:string .


###  http://www.modsem.org/fakt-news#IFCN-Code-of-Principles
fn:IFCN-Code-of-Principles rdf:type owl:NamedIndividual ,
                                    schema:CreativeWork ,
                                    fn:CodeOfPrinciples ,
                                    fn:DigitalDocument ,
                                    prov:Entity ;
                           fn:creator fn:A-1-IFCN ;
                           prov:wasAttributedTo fn:A-1-IFCN ;
                           dcterms:language "en"^^xsd:string ;
                           dcterms:title "Fact-Checking Network's code of principles"@en ;
                           schema:url "https://www.ifcncodeofprinciples.poynter.org/"^^xsd:anyURI ;
                           fn:documentContent "The code of principles of the International Fact-Checking Network at Poynter is a series of commitments organizations abide by to promote excellence in fact-checking. We believe nonpartisan and transparent fact-checking can be a powerful instrument of accountability journalism."^^xsd:string .


###  http://www.modsem.org/fakt-news#J-1
fn:J-1 rdf:type owl:NamedIndividual ,
                fn:ConfirmedFact ,
                fn:Judgment ,
                prov:Entity ;
       fn:judgmentSummary "Confirmed Fact"^^xsd:string .


###  http://www.modsem.org/fakt-news#J-2
fn:J-2 rdf:type owl:NamedIndividual ,
                fn:Judgment ,
                fn:MissingContext ,
                prov:Entity ;
       fn:judgmentSummary "Missing Context"^^xsd:string .


###  http://www.modsem.org/fakt-news#J-3
fn:J-3 rdf:type owl:NamedIndividual ,
                fn:Fabrication ,
                fn:Judgment ,
                fn:MaliciousTransfomation ,
                prov:Entity ;
       fn:judgmentSummary "Fabrication"^^xsd:string .


###  http://www.modsem.org/fakt-news#J-4
fn:J-4 rdf:type owl:NamedIndividual ,
                fn:DeceptiveEditing ,
                fn:Fabrication ,
                fn:Judgment ,
                fn:MaliciousTransfomation ,
                prov:Entity ;
       fn:judgmentSummary "Deceptive Editing"^^xsd:string .


###  http://www.modsem.org/fakt-news#Plan-R-1
fn:Plan-R-1 rdf:type owl:NamedIndividual ,
                     prov:Entity ,
                     prov:Plan ;
            fn:hasActivity fn:Activity-Evaluation-R-1 ,
                           fn:Activity-Selection-R-1 ,
                           fn:Activity-Verification-R-1 .


###  http://www.modsem.org/fakt-news#Plan-R-2
fn:Plan-R-2 rdf:type owl:NamedIndividual ,
                     prov:Entity ,
                     prov:Plan ;
            fn:hasActivity fn:Activity-Evaluation-R-2 ,
                           fn:Activity-Selection-R-2 ,
                           fn:Activity-Verification-R-2 .


###  http://www.modsem.org/fakt-news#Plan-R-3
fn:Plan-R-3 rdf:type owl:NamedIndividual ,
                     prov:Entity ,
                     prov:Plan ;
            fn:hasActivity fn:Activity-Evaluation-R-3 ,
                           fn:Activity-Selection-R-3 ,
                           fn:Activity-Verification-R-3 .


###  http://www.modsem.org/fakt-news#Plan-R-4
fn:Plan-R-4 rdf:type owl:NamedIndividual ,
                     prov:Entity ,
                     prov:Plan ;
            fn:hasActivity fn:Activity-Evaluation-R-4 ,
                           fn:Activity-Selection-R-4 ,
                           fn:Activity-Verification-R-4 .


###  http://www.modsem.org/fakt-news#R-1
fn:R-1 rdf:type owl:NamedIndividual ,
                schema:CreativeWork ,
                fn:DigitalDocument ,
                fn:Review ,
                prov:Entity ;
       fn:creator fn:A-3 ;
       fn:hasJudgment fn:J-1 ;
       fn:hasRating fn:RT-1 ;
       fn:isReviewedBy fn:A-3 ;
       fn:wasOutputOfClaimEvaluation fn:Activity-Evaluation-R-1 ;
       prov:wasAttributedTo fn:A-3 ;
       prov:wasGeneratedBy fn:Activity-Evaluation-R-1 ;
       dcterms:date "2020-10-08"^^xsd:date ;
       dcterms:language "it"^^xsd:string ;
       dcterms:title "Il governo ha davvero abolito i “decreti sicurezza”?"^^xsd:string ;
       schema:url "https://www.lavoce.info/archives/69816/il-governo-ha-davvero-abolito-i-decreti-sicurezza/"^^xsd:anyURI ;
       fn:documentContent "Il fact-checking de lavoce.info passa ...[+1283 words]"^^xsd:string ;
       fn:mention "Nicola_Zingaretti"^^xsd:string ;
       fn:reviewContent "Il fact-checking de lavoce.info passa ...[+1283 words]"^^xsd:string ;
       fn:tag "politica"^^xsd:string .


###  http://www.modsem.org/fakt-news#R-2
fn:R-2 rdf:type owl:NamedIndividual ,
                schema:CreativeWork ,
                fn:DigitalDocument ,
                fn:Review ,
                prov:Entity ;
       fn:creator fn:A-4 ;
       fn:hasJudgment fn:J-2 ;
       fn:hasRating fn:RT-2 ;
       fn:isReviewedBy fn:A-4 ;
       prov:wasAttributedTo fn:A-4 ;
       dcterms:date "2021-01-16"^^xsd:date ;
       dcterms:language "it"^^xsd:string ;
       dcterms:title "No, “genitore 1 e 2” non tornano sui documenti d’identità (non ci sono mai stati)"^^xsd:string ;
       schema:url "https://pagellapolitica.it/dichiarazioni/8801/no-genitore-1-e-2-non-tornano-sui-documenti-didentita-non-ci-sono-mai-stati"^^xsd:anyURI ;
       fn:documentContent "Al governo si preoccupano di cancellare “padre” e “madre” dalla carta di identità dei minori per sostituirli con genitore 1 e 2 ...[+1568 words]"^^xsd:string ;
       fn:mention "Matteo_Salvini"^^xsd:string ;
       fn:reviewContent "Al governo si preoccupano di cancellare “padre” e “madre” dalla carta di identità dei minori per sostituirli con genitore 1 e 2 ...[+1568 words]"^^xsd:string ;
       fn:tag "Carta d'identità"@it ,
              "Lega"@it ,
              "politica"^^xsd:string .


###  http://www.modsem.org/fakt-news#R-3
fn:R-3 rdf:type owl:NamedIndividual ,
                schema:CreativeWork ,
                fn:DigitalDocument ,
                fn:Review ,
                prov:Entity ;
       fn:creator fn:A-6 ;
       fn:hasJudgment fn:J-3 ;
       fn:hasRating fn:RT-3 ;
       fn:isReviewedBy fn:A-6 ;
       prov:wasAttributedTo fn:A-6 ;
       dcterms:date "2019-06-19"^^xsd:date ;
       dcterms:language "en"^^xsd:string ;
       dcterms:title "Facebook wouldn’t delete an altered video of Nancy Pelosi. What about one of Mark Zuckerberg?"^^xsd:string ;
       schema:url "https://www.washingtonpost.com/nation/2019/06/12/mark-zuckerberg-deepfake-facebook-instagram-nancy-pelosi/"^^xsd:anyURI ;
       fn:documentContent "A couple of short video clips, a voice actor and an artificial intelligence algorithm. That’s all two artists and a technology start-up ...[+1497 words]"^^xsd:string ;
       fn:mention "Mark_Zuckerberg"^^xsd:string ;
       fn:reviewContent "A couple of short video clips, a voice actor and an artificial intelligence algorithm. That’s all two artists and a technology start-up ...[+1497 words]"^^xsd:string ;
       fn:tag "Nancy Pelosi"^^xsd:string ,
              "deepfake"^^xsd:string .


###  http://www.modsem.org/fakt-news#R-4
fn:R-4 rdf:type owl:NamedIndividual ,
                schema:CreativeWork ,
                fn:DigitalDocument ,
                fn:Review ,
                prov:Entity ;
       fn:creator fn:A-8 ;
       fn:hasJudgment fn:J-4 ;
       fn:hasRating fn:RT-4 ;
       fn:isReviewedBy fn:A-8 ;
       prov:wasAttributedTo fn:A-8 ;
       dcterms:date "2021-01-20"^^xsd:date ;
       dcterms:language "en"^^xsd:string ;
       dcterms:title "Barack Obama wasn’t arrested before Biden’s inauguration"^^xsd:string ;
       schema:url "https://www.politifact.com/factchecks/2021/jan/18/facebook-posts/obama-wasnt-arrested-bidens-inauguration/"^^xsd:anyURI ;
       fn:documentContent "In a video published Jan. 17, Gage Nelson, host of the conservative podcast America Divided, said: \"Barack Obama was arrested.\""^^xsd:string ;
       fn:mention "Barack_Obama"^^xsd:string ,
                  "Nelson_Mandela"^^xsd:string ,
                  "QAnon"^^xsd:string ;
       fn:reviewContent "In a video published Jan. 17, Gage Nelson, host of the conservative podcast America Divided, said: \"Barack Obama was arrested.\""^^xsd:string ;
       fn:tag "politics"^^xsd:string .


###  http://www.modsem.org/fakt-news#RT-1
fn:RT-1 rdf:type owl:NamedIndividual ,
                 fn:Rating ,
                 prov:Entity ;
        schema:url "https://www.lavoce.info/come-facciamo-il-fact-checking/"^^xsd:anyURI ;
        fn:ratingSystemComment "Tendenzialmente vero"^^xsd:string ;
        fn:ratingValue "True"^^xsd:string .


###  http://www.modsem.org/fakt-news#RT-2
fn:RT-2 rdf:type owl:NamedIndividual ,
                 fn:Rating ,
                 prov:Entity ;
        schema:url "https://pagellapolitica.it/static/metodologia"^^xsd:anyURI ;
        fn:ratingSystemComment "Pinocchio andante"^^xsd:string ;
        fn:ratingValue "Mostly False"^^xsd:string .


###  http://www.modsem.org/fakt-news#RT-3
fn:RT-3 rdf:type owl:NamedIndividual ,
                 fn:Rating ,
                 prov:Entity ;
        schema:url "https://www.washingtonpost.com/graphics/2019/politics/fact-checker/manipulated-video-guide/?noredirect=on&utm_term=.985468bf6c1e&itid=lk_inline_manual_9"^^xsd:anyURI ;
        fn:ratingValue "False"^^xsd:string .


###  http://www.modsem.org/fakt-news#RT-4
fn:RT-4 rdf:type owl:NamedIndividual ,
                 fn:Rating ,
                 prov:Entity ;
        schema:url "https://www.politifact.com/article/2018/feb/12/principles-truth-o-meter-politifacts-methodology-i/#Truth-O-Meter%20ratings"^^xsd:anyURI ;
        fn:ratingAssociatedMedia "https://static.politifact.com/politifact/rulings/tom_ruling_pof.png"^^xsd:anyURI ;
        fn:ratingSystemComment "Pants On Fire"^^xsd:string ;
        fn:ratingValue "False"^^xsd:string .


###  http://www.modsem.org/fakt-news#Role-A-10
fn:Role-A-10 rdf:type owl:NamedIndividual ,
                      fn:Claimant ,
                      prov:Role .


###  http://www.modsem.org/fakt-news#Role-A-11
fn:Role-A-11 rdf:type owl:NamedIndividual ,
                      fn:Claimant ,
                      prov:Role .


###  http://www.modsem.org/fakt-news#Role-A-12
fn:Role-A-12 rdf:type owl:NamedIndividual ,
                      fn:Claimant ,
                      prov:Role .


###  http://www.modsem.org/fakt-news#Role-A-14
fn:Role-A-14 rdf:type owl:NamedIndividual ,
                      fn:Editor ,
                      prov:Role .


###  http://www.modsem.org/fakt-news#Role-A-3
fn:Role-A-3 rdf:type owl:NamedIndividual ,
                     fn:FactChecker ,
                     prov:Role .


###  http://www.modsem.org/fakt-news#Role-A-4
fn:Role-A-4 rdf:type owl:NamedIndividual ,
                     fn:FactChecker ,
                     prov:Role .


###  http://www.modsem.org/fakt-news#Role-A-6
fn:Role-A-6 rdf:type owl:NamedIndividual ,
                     fn:FactChecker ,
                     prov:Role .


###  http://www.modsem.org/fakt-news#Role-A-8
fn:Role-A-8 rdf:type owl:NamedIndividual ,
                     fn:FactChecker ,
                     prov:Role .


###  http://www.modsem.org/fakt-news#Role-A-9
fn:Role-A-9 rdf:type owl:NamedIndividual ,
                     fn:Claimant ,
                     prov:Role .


###  http://www.modsem.org/fakt-news#Time-R1-2020-10-05-2020-10-06
fn:Time-R1-2020-10-05-2020-10-06 rdf:type owl:NamedIndividual ,
                                          <http://www.ontologydesignpatterns.org/cp/owl/timeinterval.owl#TimeInterval> ,
                                          prov:Entity ;
                                 <http://www.ontologydesignpatterns.org/cp/owl/timeinterval.owl#hasIntervalDate> "2020-10-05"^^xsd:date ,
                                                                                                                 "2020-10-06"^^xsd:date ;
                                 <http://www.ontologydesignpatterns.org/cp/owl/timeinterval.owl#hasIntervalEndDate> "2020-10-06"^^xsd:date ;
                                 <http://www.ontologydesignpatterns.org/cp/owl/timeinterval.owl#hasIntervalStartDate> "2020-10-05"^^xsd:date .


###  http://www.modsem.org/fakt-news#Time-R1-2020-10-06-2020-10-07
fn:Time-R1-2020-10-06-2020-10-07 rdf:type owl:NamedIndividual ,
                                          <http://www.ontologydesignpatterns.org/cp/owl/timeinterval.owl#TimeInterval> ,
                                          prov:Entity ;
                                 <http://www.ontologydesignpatterns.org/cp/owl/timeinterval.owl#hasIntervalDate> "2020-10-06"^^xsd:date ,
                                                                                                                 "2020-10-07"^^xsd:date ;
                                 <http://www.ontologydesignpatterns.org/cp/owl/timeinterval.owl#hasIntervalEndDate> "2020-10-07"^^xsd:date ;
                                 <http://www.ontologydesignpatterns.org/cp/owl/timeinterval.owl#hasIntervalStartDate> "2020-10-06"^^xsd:date .


###  http://www.modsem.org/fakt-news#Time-R1-2020-10-07-2020-10-08
fn:Time-R1-2020-10-07-2020-10-08 rdf:type owl:NamedIndividual ,
                                          <http://www.ontologydesignpatterns.org/cp/owl/timeinterval.owl#TimeInterval> ,
                                          prov:Entity ;
                                 <http://www.ontologydesignpatterns.org/cp/owl/timeinterval.owl#hasIntervalDate> "2020-10-07"^^xsd:date ,
                                                                                                                 "2020-10-08"^^xsd:date ;
                                 <http://www.ontologydesignpatterns.org/cp/owl/timeinterval.owl#hasIntervalEndDate> "2020-10-08"^^xsd:date ;
                                 <http://www.ontologydesignpatterns.org/cp/owl/timeinterval.owl#hasIntervalStartDate> "2020-10-07"^^xsd:date .


###  http://www.modsem.org/fakt-news#Time-R2-2021-01-13-2021-01-14
fn:Time-R2-2021-01-13-2021-01-14 rdf:type owl:NamedIndividual ,
                                          <http://www.ontologydesignpatterns.org/cp/owl/timeinterval.owl#TimeInterval> ,
                                          prov:Entity ;
                                 <http://www.ontologydesignpatterns.org/cp/owl/timeinterval.owl#hasIntervalDate> "2021-01-01"^^xsd:date ,
                                                                                                                 "2021-01-13"^^xsd:date ;
                                 <http://www.ontologydesignpatterns.org/cp/owl/timeinterval.owl#hasIntervalEndDate> "2021-01-13"^^xsd:date ;
                                 <http://www.ontologydesignpatterns.org/cp/owl/timeinterval.owl#hasIntervalStartDate> "2021-01-01"^^xsd:date .


###  http://www.modsem.org/fakt-news#Time-R2-2021-01-14-2021-01-15
fn:Time-R2-2021-01-14-2021-01-15 rdf:type owl:NamedIndividual ,
                                          <http://www.ontologydesignpatterns.org/cp/owl/timeinterval.owl#TimeInterval> ,
                                          prov:Entity ;
                                 <http://www.ontologydesignpatterns.org/cp/owl/timeinterval.owl#hasIntervalDate> "2021-01-14"^^xsd:date ,
                                                                                                                 "2021-01-15"^^xsd:date ;
                                 <http://www.ontologydesignpatterns.org/cp/owl/timeinterval.owl#hasIntervalEndDate> "2021-01-15"^^xsd:date ;
                                 <http://www.ontologydesignpatterns.org/cp/owl/timeinterval.owl#hasIntervalStartDate> "2021-01-14"^^xsd:date .


###  http://www.modsem.org/fakt-news#Time-R2-2021-01-15-2021-01-16
fn:Time-R2-2021-01-15-2021-01-16 rdf:type owl:NamedIndividual ,
                                          <http://www.ontologydesignpatterns.org/cp/owl/timeinterval.owl#TimeInterval> ,
                                          prov:Entity ;
                                 <http://www.ontologydesignpatterns.org/cp/owl/timeinterval.owl#hasIntervalDate> "2021-01-15"^^xsd:date ,
                                                                                                                 "2021-01-16"^^xsd:date ;
                                 <http://www.ontologydesignpatterns.org/cp/owl/timeinterval.owl#hasIntervalEndDate> "2021-01-16"^^xsd:date ;
                                 <http://www.ontologydesignpatterns.org/cp/owl/timeinterval.owl#hasIntervalStartDate> "2021-01-15"^^xsd:date .


###  http://www.modsem.org/fakt-news#Time-R3-2019-06-16-2019-06-17
fn:Time-R3-2019-06-16-2019-06-17 rdf:type owl:NamedIndividual ,
                                          <http://www.ontologydesignpatterns.org/cp/owl/timeinterval.owl#TimeInterval> ,
                                          prov:Entity ;
                                 <http://www.ontologydesignpatterns.org/cp/owl/timeinterval.owl#hasIntervalDate> "2019-06-16"^^xsd:date ,
                                                                                                                 "2019-06-17"^^xsd:date ;
                                 <http://www.ontologydesignpatterns.org/cp/owl/timeinterval.owl#hasIntervalEndDate> "2019-06-17"^^xsd:date ;
                                 <http://www.ontologydesignpatterns.org/cp/owl/timeinterval.owl#hasIntervalStartDate> "2019-06-16"^^xsd:date .


###  http://www.modsem.org/fakt-news#Time-R3-2019-06-17-2019-06-18
fn:Time-R3-2019-06-17-2019-06-18 rdf:type owl:NamedIndividual ,
                                          <http://www.ontologydesignpatterns.org/cp/owl/timeinterval.owl#TimeInterval> ,
                                          prov:Entity ;
                                 <http://www.ontologydesignpatterns.org/cp/owl/timeinterval.owl#hasIntervalDate> "2019-06-17"^^xsd:date ,
                                                                                                                 "2019-06-18"^^xsd:date ;
                                 <http://www.ontologydesignpatterns.org/cp/owl/timeinterval.owl#hasIntervalEndDate> "2019-06-18"^^xsd:date ;
                                 <http://www.ontologydesignpatterns.org/cp/owl/timeinterval.owl#hasIntervalStartDate> "2019-06-17"^^xsd:date .


###  http://www.modsem.org/fakt-news#Time-R3-2019-06-18-2019-06-19
fn:Time-R3-2019-06-18-2019-06-19 rdf:type owl:NamedIndividual ,
                                          <http://www.ontologydesignpatterns.org/cp/owl/timeinterval.owl#TimeInterval> ,
                                          prov:Entity ;
                                 <http://www.ontologydesignpatterns.org/cp/owl/timeinterval.owl#hasIntervalDate> "2019-06-18"^^xsd:date ,
                                                                                                                 "2019-06-19"^^xsd:date ;
                                 <http://www.ontologydesignpatterns.org/cp/owl/timeinterval.owl#hasIntervalEndDate> "2019-06-19"^^xsd:date ;
                                 <http://www.ontologydesignpatterns.org/cp/owl/timeinterval.owl#hasIntervalStartDate> "2019-06-18"^^xsd:date .


###  http://www.modsem.org/fakt-news#Time-R4-2021-01-17-2021-01-18
fn:Time-R4-2021-01-17-2021-01-18 rdf:type owl:NamedIndividual ,
                                          <http://www.ontologydesignpatterns.org/cp/owl/timeinterval.owl#TimeInterval> ,
                                          prov:Entity ;
                                 <http://www.ontologydesignpatterns.org/cp/owl/timeinterval.owl#hasIntervalDate> "2021-01-17"^^xsd:date ,
                                                                                                                 "2021-01-18"^^xsd:date ;
                                 <http://www.ontologydesignpatterns.org/cp/owl/timeinterval.owl#hasIntervalEndDate> "2021-01-18"^^xsd:date ;
                                 <http://www.ontologydesignpatterns.org/cp/owl/timeinterval.owl#hasIntervalStartDate> "2021-01-17"^^xsd:date .


###  http://www.modsem.org/fakt-news#Time-R4-2021-01-18-2021-01-19
fn:Time-R4-2021-01-18-2021-01-19 rdf:type owl:NamedIndividual ,
                                          <http://www.ontologydesignpatterns.org/cp/owl/timeinterval.owl#TimeInterval> ,
                                          prov:Entity ;
                                 <http://www.ontologydesignpatterns.org/cp/owl/timeinterval.owl#hasIntervalDate> "2021-01-18"^^xsd:date ,
                                                                                                                 "2021-01-19"^^xsd:date ;
                                 <http://www.ontologydesignpatterns.org/cp/owl/timeinterval.owl#hasIntervalEndDate> "2021-01-19"^^xsd:date ;
                                 <http://www.ontologydesignpatterns.org/cp/owl/timeinterval.owl#hasIntervalStartDate> "2021-01-18"^^xsd:date .


###  http://www.modsem.org/fakt-news#Time-R4-2021-01-19-2021-01-20
fn:Time-R4-2021-01-19-2021-01-20 rdf:type owl:NamedIndividual ,
                                          <http://www.ontologydesignpatterns.org/cp/owl/timeinterval.owl#TimeInterval> ,
                                          prov:Entity ;
                                 <http://www.ontologydesignpatterns.org/cp/owl/timeinterval.owl#hasIntervalDate> "2021-01-19"^^xsd:date ,
                                                                                                                 "2021-01-20"^^xsd:date ;
                                 <http://www.ontologydesignpatterns.org/cp/owl/timeinterval.owl#hasIntervalEndDate> "2021-01-20"^^xsd:date ;
                                 <http://www.ontologydesignpatterns.org/cp/owl/timeinterval.owl#hasIntervalStartDate> "2021-01-19"^^xsd:date .


#################################################################
#    Annotations
#################################################################

dcterms:date rdfs:comment "A point or period of time associated with an event in the lifecycle of the resource."@en ;
             rdfs:label "date"@en .


#################################################################
#    General axioms
#################################################################

[ rdf:type owl:AllDisjointClasses ;
  owl:members ( fn:ClaimEvaluationActivity
                fn:SelectionActivity
                fn:VerificationActivity
              )
] .


[ rdf:type owl:AllDisjointClasses ;
  owl:members ( fn:Organization
                fn:Person
                fn:SoftwareAgent
              )
] .


[ rdf:type owl:AllDisjointClasses ;
  owl:members ( prov:Activity
                prov:Agent
                prov:Entity
              )
] .


###  Generated by the OWL API (version 4.5.9.2019-02-01T07:24:44Z) https://github.com/owlcs/owlapi
